more work on lists

src/Init/Data/List/Lemmas.lean
@@ -479,6 +479,12 @@ theorem isEmpty_false_iff_exists_mem (xs : List α) :
 theorem isEmpty_iff_length_eq_zero {l : List α} : l.isEmpty ↔ l.length = 0 := by
   rw [isEmpty_iff, length_eq_zero]
 
+@[simp] theorem isEmpty_eq_true {l : List α} : l.isEmpty ↔ l = [] := by
+  cases l <;> simp
+
+@[simp] theorem isEmpty_eq_false {l : List α} : ¬ l.isEmpty ↔ l ≠ [] := by
+  cases l <;> simp
+
 /-! ### any / all -/
 
 theorem any_eq {l : List α} : l.any p = decide (∃ x, x ∈ l ∧ p x) := by induction l <;> simp [*]
@@ -854,9 +860,11 @@ theorem exists_of_mem_map (h : b ∈ map f l) : ∃ a, a ∈ l ∧ f a = b := me
 
 theorem mem_map_of_mem (f : α → β) (h : a ∈ l) : f a ∈ map f l := mem_map.2 ⟨_, h, rfl⟩
 
-theorem forall_mem_map_iff {f : α → β} {l : List α} {P : β → Prop} :
+theorem forall_mem_map {f : α → β} {l : List α} {P : β → Prop} :
     (∀ (i) (_ : i ∈ l.map f), P i) ↔ ∀ (j) (_ : j ∈ l), P (f j) := by
   simp
+
+@[deprecated forall_mem_map (since := "2024-07-25")] abbrev forall_mem_map_iff := @forall_mem_map
 
 @[simp] theorem map_inj_left {f g : α → β} : map f l = map g l ↔ ∀ a ∈ l, f a = g a := by
   induction l <;> simp_all
@@ -890,6 +898,9 @@ theorem map_eq_cons' {f : α → β} {l : List α} :
       exact ⟨a, l₁, ⟨rfl, rfl⟩, ⟨rfl, rfl⟩⟩
     · rintro ⟨a, l₁, ⟨rfl, rfl⟩, ⟨rfl, rfl⟩⟩
       constructor <;> rfl
+
+theorem map_eq_map_iff : map f l = map g l ↔ ∀ a ∈ l, f a = g a := by
+  induction l <;> simp
 
 theorem map_eq_iff : map f l = l' ↔ ∀ i : Nat, l'[i]? = l[i]?.map f := by
   constructor
@@ -999,9 +1010,11 @@ theorem filter_length_eq_length {l} : (filter p l).length = l.length ↔ ∀ a �
 theorem filter_eq_nil {l} : filter p l = [] ↔ ∀ a, a ∈ l → ¬p a := by
   simp only [eq_nil_iff_forall_not_mem, mem_filter, not_and]
 
-theorem forall_mem_filter_iff {l : List α} {p : α → Bool} {P : α → Prop} :
+theorem forall_mem_filter {l : List α} {p : α → Bool} {P : α → Prop} :
     (∀ (i) (_ : i ∈ l.filter p), P i) ↔ ∀ (j) (_ : j ∈ l), p j → P j := by
   simp
+
+@[deprecated forall_mem_filter (since := "2024-07-25")] abbrev forall_mem_filter_iff := @forall_mem_filter
 
 @[simp] theorem filter_filter (q) : ∀ l, filter p (filter q l) = filter (fun a => p a ∧ q a) l
   | [] => rfl
@@ -1143,13 +1156,15 @@ theorem filterMap_filter (p : α → Bool) (f : α → Option β) (l : List α) 
     b ∈ filterMap f l ↔ ∃ a, a ∈ l ∧ f a = some b := by
   induction l <;> simp [filterMap_cons]; split <;> simp [*, eq_comm]
 
-theorem forall_mem_filterMap_iff {f : α → Option β} {l : List α} {P : β → Prop} :
+theorem forall_mem_filterMap {f : α → Option β} {l : List α} {P : β → Prop} :
     (∀ (i) (_ : i ∈ filterMap f l), P i) ↔ ∀ (j) (_ : j ∈ l) (b), f j = some b → P b := by
   simp only [mem_filterMap, forall_exists_index, and_imp]
   rw [forall_comm]
   apply forall_congr'
   intro a
   rw [forall_comm]
+
+@[deprecated forall_mem_filterMap (since := "2024-07-25")] abbrev forall_mem_filterMap_iff := @forall_mem_filterMap
 
 @[simp] theorem filterMap_append {α β : Type _} (l l' : List α) (f : α → Option β) :
     filterMap f (l ++ l') = filterMap f l ++ filterMap f l' := by
@@ -1507,6 +1522,11 @@ theorem exists_of_mem_join : a ∈ join L → ∃ l, l ∈ L ∧ a ∈ l := mem_
 
 theorem mem_join_of_mem (lL : l ∈ L) (al : a ∈ l) : a ∈ join L := mem_join.2 ⟨l, lL, al⟩
 
+theorem forall_mem_join {p : α → Prop} {L : List (List α)} :
+    (∀ (x) (_ : x ∈ join L), p x) ↔ ∀ (l) (_ : l ∈ L) (x) (_ : x ∈ l), p x := by
+  simp only [mem_join, forall_exists_index, and_imp]
+  constructor <;> (intros; solve_by_elim)
+
 theorem join_eq_bind {L : List (List α)} : join L = L.bind id := by
   induction L <;> simp [List.bind]
 
@@ -1547,23 +1567,6 @@ theorem join_concat (L : List (List α)) (l : List α) : join (L ++ [l]) = join 
 theorem join_join {L : List (List (List α))} : join (join L) = join (map join L) := by
   induction L <;> simp_all
 
-theorem join_eq_join_iff {L L' : List (List α)} :
-    L.join = L'.join ↔ ∃ (M M' : List (List (List α))), M.map join = L ∧ M'.map join = L' ∧ M.join = M'.join := by
-  constructor
-  · intro h
-    induction L' generalizing L with
-    | nil =>
-      simp at h
-      simp
-      refine ⟨L.map fun _ => [], ?_⟩
-      simp [map_]
-      sorry
-    | cons l L' ih =>
-      simp at h
-      sorry
-  · rintro ⟨M, M', rfl, rfl, w⟩
-    simp [← join_join, w]
-#exit
 /-! ### bind -/
 
 theorem bind_def (l : List α) (f : α → List β) : l.bind f = join (map f l) := by rfl
@@ -1579,6 +1582,11 @@ theorem exists_of_mem_bind {b : β} {l : List α} {f : α → List β} :
 
 theorem mem_bind_of_mem {b : β} {l : List α} {f : α → List β} {a} (al : a ∈ l) (h : b ∈ f a) :
     b ∈ l.bind f := mem_bind.2 ⟨a, al, h⟩
+
+theorem forall_mem_bind {p : β → Prop} {l : List α} {f : α → List β} :
+    (∀ (x) (_ : x ∈ l.bind f), p x) ↔ ∀ (a) (_ : a ∈ l) (b) (_ : b ∈ f a), p b := by
+  simp only [mem_bind, forall_exists_index, and_imp]
+  constructor <;> (intros; solve_by_elim)
 
 theorem bind_singleton (f : α → List β) (x : α) : [x].bind f = f x :=
   append_nil (f x)
@@ -1654,6 +1662,10 @@ theorem bind_eq_foldl (f : α → List β) (l : List α) :
   | n+1 => by simp [replicate_succ, mem_replicate, Nat.succ_ne_zero]
 
 theorem eq_of_mem_replicate {a b : α} {n} (h : b ∈ replicate n a) : b = a := (mem_replicate.1 h).2
+
+theorem forall_mem_replicate {p : α → Prop} {a : α} {n} :
+    (∀ b, b ∈ replicate n a → p b) ↔ n = 0 ∨ p a := by
+  cases n <;> simp [mem_replicate]
 
 @[simp] theorem replicate_succ_ne_nil (n : Nat) (a : α) : replicate (n+1) a ≠ [] := by
   simp [replicate_succ]
@@ -1795,6 +1807,17 @@ theorem bind_replicate {β} (f : α → List β) : (replicate n a).bind f = (rep
   | nil => rfl
   | cons a as ih => simp [ih]
 
+@[simp] theorem mem_reverseAux {x : α} : ∀ {as bs}, x ∈ reverseAux as bs ↔ x ∈ as ∨ x ∈ bs
+  | [], _ => ⟨.inr, fun | .inr h => h⟩
+  | a :: _, _ => by rw [reverseAux, mem_cons, or_assoc, or_left_comm, mem_reverseAux, mem_cons]
+
+@[simp] theorem mem_reverse {x : α} {as : List α} : x ∈ reverse as ↔ x ∈ as := by simp [reverse]
+
+@[simp] theorem reverse_eq_nil_iff {xs : List α} : xs.reverse = [] ↔ xs = [] := by
+  match xs with
+  | [] => simp
+  | x :: xs => simp
+
 theorem getElem?_reverse' : ∀ {l : List α} (i j), i + j + 1 = length l →
     l.reverse[i]? = l[j]?
   | [], _, _, _ => rfl
@@ -1827,13 +1850,13 @@ theorem reverseAux_reverseAux_nil (as bs : List α) : reverseAux (reverseAux as 
 @[simp] theorem reverse_reverse (as : List α) : as.reverse.reverse = as := by
   simp only [reverse]; rw [reverseAux_reverseAux_nil]; rfl
 
+theorem reverse_eq_iff {as bs : List α} : as.reverse = bs ↔ as = bs.reverse := by
+  constructor <;> (rintro rfl; simp)
+
 @[simp] theorem getLast?_reverse (l : List α) : l.reverse.getLast? = l.head? := by cases l <;> simp
 
 @[simp] theorem head?_reverse (l : List α) : l.reverse.head? = l.getLast? := by
   rw [← getLast?_reverse, reverse_reverse]
-
-@[simp] theorem reverse_append (as bs : List α) : (as ++ bs).reverse = bs.reverse ++ as.reverse := by
-  induction as <;> simp_all
 
 @[simp] theorem map_reverse (f : α → β) (l : List α) : l.reverse.map f = (l.map f).reverse := by
   induction l <;> simp [*]
@@ -1856,6 +1879,12 @@ theorem reverse_map (f : α → β) (l : List α) : (l.map f).reverse = l.revers
     simp only [reverse_cons, filterMap_append, filterMap_cons, ih]
     split <;> simp_all
 
+@[simp] theorem reverse_append (as bs : List α) : (as ++ bs).reverse = bs.reverse ++ as.reverse := by
+  induction as <;> simp_all
+
+theorem reverse_concat (l : List α) (a : α) : (l.concat a).reverse = a :: l.reverse := by
+  rw [concat_eq_append, reverse_append]; rfl
+
 /-- Reversing a join is the same as reversing the order of parts and reversing all parts. -/
 theorem reverse_join (L : List (List α)) :
     L.join.reverse = (L.map reverse).reverse.join := by
@@ -1871,17 +1900,6 @@ theorem reverse_bind {β} (l : List α) (f : α → List β) : (l.bind f).revers
 
 theorem bind_reverse {β} (l : List α) (f : α → List β) : (l.reverse.bind f) = (l.bind (reverse ∘ f)).reverse := by
   induction l <;> simp_all
-
-@[simp] theorem reverse_eq_nil_iff {xs : List α} : xs.reverse = [] ↔ xs = [] := by
-  match xs with
-  | [] => simp
-  | x :: xs => simp
-
-@[simp] theorem mem_reverseAux {x : α} : ∀ {as bs}, x ∈ reverseAux as bs ↔ x ∈ as ∨ x ∈ bs
-  | [], _ => ⟨.inr, fun | .inr h => h⟩
-  | a :: _, _ => by rw [reverseAux, mem_cons, or_assoc, or_left_comm, mem_reverseAux, mem_cons]
-
-@[simp] theorem mem_reverse {x : α} {as : List α} : x ∈ reverse as ↔ x ∈ as := by simp [reverse]
 
 theorem reverseAux_eq (as bs : List α) : reverseAux as bs = reverse as ++ bs :=
   reverseAux_eq_append ..
@@ -2034,124 +2052,6 @@ theorem lt_length_of_take_ne_self {l : List α} {n} (h : l.take n ≠ l) : n < l
 
 @[simp] theorem take_length (l : List α) : take l.length l = l := take_of_length_le (Nat.le_refl _)
 
-theorem take_concat_get (l : List α) (i : Nat) (h : i < l.length) :
-    (l.take i).concat l[i] = l.take (i+1) :=
-  Eq.symm <| (append_left_inj _).1 <| (take_append_drop (i+1) l).trans <| by
-    rw [concat_eq_append, append_assoc, singleton_append, get_drop_eq_drop, take_append_drop]
-
-theorem reverse_concat (l : List α) (a : α) : (l.concat a).reverse = a :: l.reverse := by
-  rw [concat_eq_append, reverse_append]; rfl
-
-abbrev take_succ_cons := @take_cons_succ
-
-theorem take_all_of_le {n} {l : List α} (h : length l ≤ n) : take n l = l :=
-  take_of_length_le h
-
-@[simp]
-theorem take_left : ∀ l₁ l₂ : List α, take (length l₁) (l₁ ++ l₂) = l₁
-  | [], _ => rfl
-  | a :: l₁, l₂ => congrArg (cons a) (take_left l₁ l₂)
-
-theorem take_left' {l₁ l₂ : List α} {n} (h : length l₁ = n) : take n (l₁ ++ l₂) = l₁ := by
-  rw [← h]; apply take_left
-
-@[simp] theorem map_take (f : α → β) :
-    ∀ (L : List α) (i : Nat), (L.take i).map f = (L.map f).take i
-  | [], i => by simp
-  | _, 0 => by simp
-  | h :: t, n + 1 => by dsimp; rw [map_take f t n]
-
-theorem getElem?_take {l : List α} {n m : Nat} (h : m < n) : (l.take n)[m]? = l[m]? := by
-  induction n generalizing l m with
-  | zero =>
-    exact absurd h (Nat.not_lt_of_le m.zero_le)
-  | succ _ hn =>
-    cases l with
-    | nil => simp only [take_nil]
-    | cons hd tl =>
-      cases m
-      · simp
-      · simpa using hn (Nat.lt_of_succ_lt_succ h)
-
-@[deprecated getElem?_take (since := "2024-06-12")]
-theorem get?_take {l : List α} {n m : Nat} (h : m < n) : (l.take n).get? m = l.get? m := by
-  simp [getElem?_take, h]
-
-@[simp]
-theorem get?_take_of_succ {l : List α} {n : Nat} : (l.take (n + 1))[n]? = l[n]? :=
-  getElem?_take (Nat.lt_succ_self n)
-
-theorem take_succ {l : List α} {n : Nat} : l.take (n + 1) = l.take n ++ l[n]?.toList := by
-  induction l generalizing n with
-  | nil =>
-    simp only [take_nil, Option.toList, getElem?_nil, append_nil]
-  | cons hd tl hl =>
-    cases n
-    · simp only [take, Option.toList, getElem?_cons_zero, nil_append]
-    · simp only [take, hl, getElem?_cons_succ, cons_append]
-
-@[simp]
-theorem take_eq_nil_iff {l : List α} {k : Nat} : l.take k = [] ↔ l = [] ∨ k = 0 := by
-  cases l <;> cases k <;> simp [Nat.succ_ne_zero]
-
-theorem take_eq_nil_of_eq_nil : ∀ {as : List α} {i}, as = [] → as.take i = []
-  | _, _, rfl => take_nil
-
-theorem ne_nil_of_take_ne_nil {as : List α} {i : Nat} (h: as.take i ≠ []) : as ≠ [] :=
-  mt take_eq_nil_of_eq_nil h
-
-theorem dropLast_eq_take (l : List α) : l.dropLast = l.take l.length.pred := by
-  cases l with
-  | nil => simp [dropLast]
-  | cons x l =>
-    induction l generalizing x with
-    | nil => simp [dropLast]
-    | cons hd tl hl => simp [dropLast, hl]
-
-@[simp]
-theorem drop_eq_nil_iff_le {l : List α} {k : Nat} : l.drop k = [] ↔ l.length ≤ k := by
-  refine' ⟨fun h => _, drop_eq_nil_of_le⟩
-  induction k generalizing l with
-  | zero =>
-    simp only [drop] at h
-    simp [h]
-  | succ k hk =>
-    cases l
-    · simp
-    · simp only [drop] at h
-      simpa [Nat.succ_le_succ_iff] using hk h
-
-theorem drop_sizeOf_le [SizeOf α] (l : List α) (n : Nat) : sizeOf (l.drop n) ≤ sizeOf l := by
-  induction l generalizing n with
-  | nil => rw [drop_nil]; apply Nat.le_refl
-  | cons _ _ lih =>
-    induction n with
-    | zero => apply Nat.le_refl
-    | succ n =>
-      exact Trans.trans (lih _) (Nat.le_add_left _ _)
-
-@[simp] theorem drop_drop (n : Nat) : ∀ (m) (l : List α), drop n (drop m l) = drop (n + m) l
-  | m, [] => by simp
-  | 0, l => by simp
-  | m + 1, a :: l =>
-    calc
-      drop n (drop (m + 1) (a :: l)) = drop n (drop m l) := rfl
-      _ = drop (n + m) l := drop_drop n m l
-      _ = drop (n + (m + 1)) (a :: l) := rfl
-
-theorem take_drop : ∀ (m n : Nat) (l : List α), take n (drop m l) = drop m (take (m + n) l)
-  | 0, _, _ => by simp
-  | _, _, [] => by simp
-  | _+1, _, _ :: _ => by simpa [Nat.succ_add, take_succ_cons, drop_succ_cons] using take_drop ..
-
-@[simp] theorem map_drop (f : α → β) :
-    ∀ (L : List α) (i : Nat), (L.drop i).map f = (L.map f).drop i
-  | [], i => by simp
-  | L, 0 => by simp
-  | h :: t, n + 1 => by
-    dsimp
-    rw [map_drop f t]
-
 @[simp]
 theorem getElem_cons_drop : ∀ (l : List α) (i : Nat) (h : i < l.length),
     l[i] :: drop (i + 1) l = drop i l
@@ -2169,23 +2069,168 @@ theorem drop_eq_getElem_cons {n} {l : List α} (h) : drop n l = l[n] :: drop (n 
 theorem drop_eq_get_cons {n} {l : List α} (h) : drop n l = get l ⟨n, h⟩ :: drop (n + 1) l := by
   simp [drop_eq_getElem_cons]
 
+@[simp]
+theorem getElem?_take {l : List α} {n m : Nat} (h : m < n) : (l.take n)[m]? = l[m]? := by
+  induction n generalizing l m with
+  | zero =>
+    exact absurd h (Nat.not_lt_of_le m.zero_le)
+  | succ _ hn =>
+    cases l with
+    | nil => simp only [take_nil]
+    | cons hd tl =>
+      cases m
+      · simp
+      · simpa using hn (Nat.lt_of_succ_lt_succ h)
+
+@[deprecated getElem?_take (since := "2024-06-12")]
+theorem get?_take {l : List α} {n m : Nat} (h : m < n) : (l.take n).get? m = l.get? m := by
+  simp [getElem?_take, h]
+
+@[simp]
+theorem getElem?_take_of_succ {l : List α} {n : Nat} : (l.take (n + 1))[n]? = l[n]? :=
+  getElem?_take (Nat.lt_succ_self n)
+
+@[simp]
+theorem drop_eq_nil_iff_le {l : List α} {k : Nat} : l.drop k = [] ↔ l.length ≤ k := by
+  refine' ⟨fun h => _, drop_eq_nil_of_le⟩
+  induction k generalizing l with
+  | zero =>
+    simp only [drop] at h
+    simp [h]
+  | succ k hk =>
+    cases l
+    · simp
+    · simp only [drop] at h
+      simpa [Nat.succ_le_succ_iff] using hk h
+
+@[simp]
+theorem take_eq_nil_iff {l : List α} {k : Nat} : l.take k = [] ↔ k = 0 ∨ l = [] := by
+  cases l <;> cases k <;> simp [Nat.succ_ne_zero]
+
 theorem drop_eq_nil_of_eq_nil : ∀ {as : List α} {i}, as = [] → as.drop i = []
   | _, _, rfl => drop_nil
 
 theorem ne_nil_of_drop_ne_nil {as : List α} {i : Nat} (h: as.drop i ≠ []) : as ≠ [] :=
   mt drop_eq_nil_of_eq_nil h
 
-@[deprecated drop_drop (since := "2024-06-15")]
-theorem drop_add (m n) (l : List α) : drop (m + n) l = drop m (drop n l) := by
-  simp [drop_drop]
+theorem take_eq_nil_of_eq_nil : ∀ {as : List α} {i}, as = [] → as.take i = []
+  | _, _, rfl => take_nil
 
-@[simp]
+theorem ne_nil_of_take_ne_nil {as : List α} {i : Nat} (h : as.take i ≠ []) : as ≠ [] :=
+  mt take_eq_nil_of_eq_nil h
+
+theorem set_take {l : List α} {n m : Nat} {a : α} :
+    (l.set m a).take n = (l.take n).set m a := by
+  induction n generalizing l m with
+  | zero => simp
+  | succ _ hn =>
+    cases l with
+    | nil => simp
+    | cons hd tl => cases m <;> simp_all
+
+theorem drop_set {l : List α} {n m : Nat} {a : α} :
+    (l.set m a).drop n = if m < n then l.drop n else (l.drop n).set (m - n) a := by
+  induction n generalizing l m with
+  | zero => simp
+  | succ _ hn =>
+    cases l with
+    | nil => simp
+    | cons hd tl =>
+      cases m
+      · simp_all
+      · simp only [hn, set_cons_succ, drop_succ_cons, succ_lt_succ_iff]
+        congr 2
+        exact (Nat.add_sub_add_right ..).symm
+
+theorem set_drop {l : List α} {n m : Nat} {a : α} :
+    (l.drop n).set m a = (l.set (n + m) a).drop n := by
+  rw [drop_set, if_neg, add_sub_self_left n m]
+  exact (Nat.not_lt).2 (le_add_right n m)
+
+theorem take_concat_get (l : List α) (i : Nat) (h : i < l.length) :
+    (l.take i).concat l[i] = l.take (i+1) :=
+  Eq.symm <| (append_left_inj _).1 <| (take_append_drop (i+1) l).trans <| by
+    rw [concat_eq_append, append_assoc, singleton_append, get_drop_eq_drop, take_append_drop]
+
+@[deprecated (since := "2024-07-25")]
+theorem take_cons_succ : (a::as).take (i+1) = a :: as.take i := rfl
+
+@[deprecated (since := "2024-07-25")]
+theorem take_all_of_le {n} {l : List α} (h : length l ≤ n) : take n l = l :=
+  take_of_length_le h
+
 theorem drop_left : ∀ l₁ l₂ : List α, drop (length l₁) (l₁ ++ l₂) = l₂
   | [], _ => rfl
   | _ :: l₁, l₂ => drop_left l₁ l₂
 
+@[simp]
 theorem drop_left' {l₁ l₂ : List α} {n} (h : length l₁ = n) : drop n (l₁ ++ l₂) = l₂ := by
   rw [← h]; apply drop_left
+
+theorem take_left : ∀ l₁ l₂ : List α, take (length l₁) (l₁ ++ l₂) = l₁
+  | [], _ => rfl
+  | a :: l₁, l₂ => congrArg (cons a) (take_left l₁ l₂)
+
+@[simp]
+theorem take_left' {l₁ l₂ : List α} {n} (h : length l₁ = n) : take n (l₁ ++ l₂) = l₁ := by
+  rw [← h]; apply take_left
+
+theorem take_succ {l : List α} {n : Nat} : l.take (n + 1) = l.take n ++ l[n]?.toList := by
+  induction l generalizing n with
+  | nil =>
+    simp only [take_nil, Option.toList, getElem?_nil, append_nil]
+  | cons hd tl hl =>
+    cases n
+    · simp only [take, Option.toList, getElem?_cons_zero, nil_append]
+    · simp only [take, hl, getElem?_cons_succ, cons_append]
+
+@[deprecated (since := "2024-07-25")]
+theorem drop_sizeOf_le [SizeOf α] (l : List α) (n : Nat) : sizeOf (l.drop n) ≤ sizeOf l := by
+  induction l generalizing n with
+  | nil => rw [drop_nil]; apply Nat.le_refl
+  | cons _ _ lih =>
+    induction n with
+    | zero => apply Nat.le_refl
+    | succ n =>
+      exact Trans.trans (lih _) (Nat.le_add_left _ _)
+
+theorem dropLast_eq_take (l : List α) : l.dropLast = l.take (l.length - 1) := by
+  cases l with
+  | nil => simp [dropLast]
+  | cons x l =>
+    induction l generalizing x <;> simp_all [dropLast]
+
+@[simp] theorem map_take (f : α → β) :
+    ∀ (L : List α) (i : Nat), (L.take i).map f = (L.map f).take i
+  | [], i => by simp
+  | _, 0 => by simp
+  | h :: t, n + 1 => by dsimp; rw [map_take f t n]
+
+@[simp] theorem map_drop (f : α → β) :
+    ∀ (L : List α) (i : Nat), (L.drop i).map f = (L.map f).drop i
+  | [], i => by simp
+  | L, 0 => by simp
+  | h :: t, n + 1 => by
+    dsimp
+    rw [map_drop f t]
+
+@[simp] theorem drop_drop (n : Nat) : ∀ (m) (l : List α), drop n (drop m l) = drop (n + m) l
+  | m, [] => by simp
+  | 0, l => by simp
+  | m + 1, a :: l =>
+    calc
+      drop n (drop (m + 1) (a :: l)) = drop n (drop m l) := rfl
+      _ = drop (n + m) l := drop_drop n m l
+      _ = drop (n + (m + 1)) (a :: l) := rfl
+
+theorem take_drop : ∀ (m n : Nat) (l : List α), take n (drop m l) = drop m (take (m + n) l)
+  | 0, _, _ => by simp
+  | _, _, [] => by simp
+  | _+1, _, _ :: _ => by simpa [Nat.succ_add, take_succ_cons, drop_succ_cons] using take_drop ..
+
+@[deprecated drop_drop (since := "2024-06-15")]
+theorem drop_add (m n) (l : List α) : drop (m + n) l = drop m (drop n l) := by
+  simp [drop_drop]
 
 /-! ### takeWhile and dropWhile -/
 
@@ -2258,6 +2303,38 @@ theorem dropWhile_map (f : α → β) (p : β → Bool) (l : List α) :
     simp only [map_cons, dropWhile_cons]
     split <;> simp_all
 
+theorem takeWhile_filterMap (f : α → Option β) (p : β → Bool) (l : List α) :
+    (l.filterMap f).takeWhile p = (l.takeWhile fun a => (f a).all p).filterMap f := by
+  induction l with
+  | nil => rfl
+  | cons x xs ih =>
+    simp only [filterMap_cons]
+    split <;> rename_i h
+    · simp only [takeWhile_cons, h]
+      split <;> simp_all
+    · simp [takeWhile_cons, h, ih]
+      split <;> simp_all [filterMap_cons]
+
+theorem dropWhile_filterMap (f : α → Option β) (p : β → Bool) (l : List α) :
+    (l.filterMap f).dropWhile p = (l.dropWhile fun a => (f a).all p).filterMap f := by
+  induction l with
+  | nil => rfl
+  | cons x xs ih =>
+    simp only [filterMap_cons]
+    split <;> rename_i h
+    · simp only [dropWhile_cons, h]
+      split <;> simp_all
+    · simp [dropWhile_cons, h, ih]
+      split <;> simp_all [filterMap_cons]
+
+theorem takeWhile_filter (p q : α → Bool) (l : List α) :
+    (l.filter p).takeWhile q = (l.takeWhile fun a => !p a || q a).filter p := by
+  simp [← filterMap_eq_filter, takeWhile_filterMap]
+
+theorem dropWhile_filter (p q : α → Bool) (l : List α) :
+    (l.filter p).dropWhile q = (l.dropWhile fun a => !p a || q a).filter p := by
+  simp [← filterMap_eq_filter, dropWhile_filterMap]
+
 @[simp] theorem takeWhile_append_dropWhile (p : α → Bool) :
     ∀ (l : List α), takeWhile p l ++ dropWhile p l = l
   | [] => rfl
@@ -2321,14 +2398,29 @@ theorem dropWhile_replicate (p : α → Bool) :
   simp only [dropWhile_replicate_eq_filter_not, filter_replicate]
   split <;> simp_all
 
-/-! ### partition -/
+theorem take_takeWhile {l : List α} (p : α → Bool) n :
+    (l.takeWhile p).take n = (l.takeWhile p).take n := by
+  induction l with
+  | nil => rfl
+  | cons x xs ih =>
+    by_cases h : p x <;> simp [takeWhile_cons, h, ih]
+
+/-! ### partition
+
+Because we immediately simplify `partition` into two `filter`s for verification purposes,
+we do not separately develop much theory about it.
+-/
 
 @[simp] theorem partition_eq_filter_filter (p : α → Bool) (l : List α) :
-    partition p l = (filter p l, filter (not ∘ p) l) := by simp [partition, aux] where
-  aux : ∀ l {as bs}, partition.loop p l (as, bs) =
-    (as.reverse ++ filter p l, bs.reverse ++ filter (not ∘ p) l)
-  | [] => by simp [partition.loop, filter]
-  | a :: l => by cases pa : p a <;> simp [partition.loop, pa, aux, filter, append_assoc]
+    partition p l = (filter p l, filter (not ∘ p) l) := by simp [partition, aux]
+  where
+    aux : ∀ l {as bs}, partition.loop p l (as, bs) =
+        (as.reverse ++ filter p l, bs.reverse ++ filter (not ∘ p) l)
+      | [] => by simp [partition.loop, filter]
+      | a :: l => by cases pa : p a <;> simp [partition.loop, pa, aux, filter, append_assoc]
+
+theorem mem_partition : a ∈ l ↔ a ∈ (partition p l).1 ∨ a ∈ (partition p l).2 := by
+  by_cases p a <;> simp_all
 
 /-! ### dropLast
 
@@ -2350,9 +2442,38 @@ theorem get_dropLast (xs : List α) (i : Fin xs.dropLast.length) :
     xs.dropLast.get i = xs.get ⟨i, Nat.lt_of_lt_of_le i.isLt (length_dropLast .. ▸ Nat.pred_le _)⟩ := by
   simp
 
+theorem getElem?_dropLast (xs : List α) (i : Nat) :
+    xs.dropLast[i]? = if i < xs.length - 1 then xs[i]? else none := by
+  split
+  · rw [getElem?_eq_getElem, getElem?_eq_getElem, getElem_dropLast]
+    simpa
+  · simp_all
+
+theorem head_dropLast (xs : List α) (h) :
+    xs.dropLast.head h = xs.head (by rintro rfl; simp at h) := by
+  cases xs with
+  | nil => rfl
+  | cons x xs =>
+    cases xs with
+    | nil => simp at h
+    | cons y ys => rfl
+
+theorem head?_dropLast (xs : List α) : xs.dropLast.head? = if 1 < xs.length then xs.head? else none := by
+  cases xs with
+  | nil => rfl
+  | cons x xs =>
+    cases xs with
+    | nil => rfl
+    | cons y ys => simp [Nat.succ_lt_succ_iff]
+
 theorem dropLast_cons_of_ne_nil {α : Type u} {x : α}
     {l : List α} (h : l ≠ []) : (x :: l).dropLast = x :: l.dropLast := by
   simp [dropLast, h]
+
+@[simp] theorem map_dropLast (f : α → β) (l : List α) : l.dropLast.map f = (l.map f).dropLast := by
+  induction l with
+  | nil => rfl
+  | cons x xs ih => cases xs <;> simp [ih]
 
 @[simp] theorem dropLast_append_of_ne_nil {α : Type u} {l : List α} :
     ∀ (l' : List α) (_ : l ≠ []), (l' ++ l).dropLast = l' ++ l.dropLast
@@ -2361,15 +2482,14 @@ theorem dropLast_cons_of_ne_nil {α : Type u} {x : α}
     rw [cons_append, dropLast, dropLast_append_of_ne_nil l' h, cons_append]
     simp [h]
 
-theorem dropLast_append_cons : dropLast (l₁ ++ b::l₂) = l₁ ++ dropLast (b::l₂) := by
+theorem dropLast_append {l₁ l₂ : List α} :
+    (l₁ ++ l₂).dropLast = if l₂.isEmpty then l₁.dropLast else l₁ ++ l₂.dropLast := by
+  split <;> simp_all
+
+@[simp] theorem dropLast_append_cons : dropLast (l₁ ++ b::l₂) = l₁ ++ dropLast (b::l₂) := by
   simp only [ne_eq, not_false_eq_true, dropLast_append_of_ne_nil]
 
 @[simp 1100] theorem dropLast_concat : dropLast (l₁ ++ [b]) = l₁ := by simp
-
-@[simp] theorem map_dropLast (f : α → β) (l : List α) : l.dropLast.map f = (l.map f).dropLast := by
-  induction l with
-  | nil => rfl
-  | cons x xs ih => cases xs <;> simp [ih]
 
 @[simp] theorem dropLast_replicate (n) (a : α) : dropLast (replicate n a) = replicate (n - 1) a := by
   match n with
@@ -2437,7 +2557,7 @@ instance : Trans (Membership.mem : α → List α → Prop) Subset Membership.me
 instance : Trans (Subset : List α → List α → Prop) Subset Subset :=
   ⟨Subset.trans⟩
 
-@[simp] theorem subset_cons (a : α) (l : List α) : l ⊆ a :: l := fun _ => Mem.tail _
+@[simp] theorem subset_cons_self (a : α) (l : List α) : l ⊆ a :: l := fun _ => Mem.tail _
 
 theorem subset_of_cons_subset {a : α} {l₁ l₂ : List α} : a :: l₁ ⊆ l₂ → l₁ ⊆ l₂ :=
   fun s _ i => s (mem_cons_of_mem _ i)
@@ -2447,6 +2567,25 @@ theorem subset_cons_of_subset (a : α) {l₁ l₂ : List α} : l₁ ⊆ l₂ →
 
 theorem cons_subset_cons {l₁ l₂ : List α} (a : α) (s : l₁ ⊆ l₂) : a :: l₁ ⊆ a :: l₂ :=
   fun _ => by simp only [mem_cons]; exact Or.imp_right (@s _)
+
+@[simp] theorem cons_subset : a :: l ⊆ m ↔ a ∈ m ∧ l ⊆ m := by
+  simp only [subset_def, mem_cons, or_imp, forall_and, forall_eq]
+
+@[simp] theorem subset_nil {l : List α} : l ⊆ [] ↔ l = [] :=
+  ⟨fun h => match l with | [] => rfl | _::_ => (nomatch h (.head ..)), fun | rfl => Subset.refl _⟩
+
+theorem map_subset {l₁ l₂ : List α} (f : α → β) (H : l₁ ⊆ l₂) : map f l₁ ⊆ map f l₂ :=
+  fun x => by simp only [mem_map]; exact .imp fun a => .imp_left (@H _)
+
+theorem filter_subset {l₁ l₂ : List α} (p : α → Bool) (H : l₁ ⊆ l₂) : filter p l₁ ⊆ filter p l₂ :=
+  fun x => by simp_all [mem_filter, subset_def.1 H]
+
+theorem filterMap_subset {l₁ l₂ : List α} (f : α → Option β) (H : l₁ ⊆ l₂) :
+    filterMap f l₁ ⊆ filterMap f l₂ := by
+  intro x
+  simp only [mem_filterMap]
+  rintro ⟨a, h, w⟩
+  exact ⟨a, H h, w⟩
 
 @[simp] theorem subset_append_left (l₁ l₂ : List α) : l₁ ⊆ l₁ ++ l₂ := fun _ => mem_append_left _
 
@@ -2458,17 +2597,27 @@ fun s => Subset.trans s <| subset_append_left _ _
 theorem subset_append_of_subset_right (l₁ : List α) : l ⊆ l₂ → l ⊆ l₁ ++ l₂ :=
 fun s => Subset.trans s <| subset_append_right _ _
 
-@[simp] theorem cons_subset : a :: l ⊆ m ↔ a ∈ m ∧ l ⊆ m := by
-  simp only [subset_def, mem_cons, or_imp, forall_and, forall_eq]
-
 @[simp] theorem append_subset {l₁ l₂ l : List α} :
     l₁ ++ l₂ ⊆ l ↔ l₁ ⊆ l ∧ l₂ ⊆ l := by simp [subset_def, or_imp, forall_and]
 
-theorem subset_nil {l : List α} : l ⊆ [] ↔ l = [] :=
-  ⟨fun h => match l with | [] => rfl | _::_ => (nomatch h (.head ..)), fun | rfl => Subset.refl _⟩
+theorem replicate_subset {n : Nat} {a : α} {l : List α} : replicate n a ⊆ l ↔ n = 0 ∨ a ∈ l := by
+  induction n with
+  | zero => simp
+  | succ n ih => simp (config := {contextual := true}) [replicate_succ, ih, cons_subset]
 
-theorem map_subset {l₁ l₂ : List α} (f : α → β) (H : l₁ ⊆ l₂) : map f l₁ ⊆ map f l₂ :=
-  fun x => by simp only [mem_map]; exact .imp fun a => .imp_left (@H _)
+theorem subset_replicate {n : Nat} {a : α} {l : List α} (h : n ≠ 0) : l ⊆ replicate n a ↔ ∀ x ∈ l, x = a := by
+  induction l with
+  | nil => simp
+  | cons x xs ih =>
+    simp only [cons_subset, mem_replicate, ne_eq, ih, mem_cons, forall_eq_or_imp,
+      and_congr_left_iff, and_iff_right_iff_imp]
+    solve_by_elim
+
+@[simp] theorem reverse_subset {l₁ l₂ : List α} : reverse l₁ ⊆ l₂ ↔ l₁ ⊆ l₂ := by
+  simp [subset_def]
+
+@[simp] theorem subset_reverse {l₁ l₂ : List α} : l₁ ⊆ reverse l₂ ↔ l₁ ⊆ l₂ := by
+  simp [subset_def]
 
 /-! ### Sublist and isSublist -/
 
@@ -2493,10 +2642,10 @@ theorem Sublist.trans {l₁ l₂ l₃ : List α} (h₁ : l₁ <+ l₂) (h₂ : l
 
 instance : Trans (@Sublist α) Sublist Sublist := ⟨Sublist.trans⟩
 
-@[simp] theorem sublist_cons (a : α) (l : List α) : l <+ a :: l := (Sublist.refl l).cons _
+@[simp] theorem sublist_cons_self (a : α) (l : List α) : l <+ a :: l := (Sublist.refl l).cons _
 
 theorem sublist_of_cons_sublist : a :: l₁ <+ l₂ → l₁ <+ l₂ :=
-  (sublist_cons a l₁).trans
+  (sublist_cons_self a l₁).trans
 
 @[simp]
 theorem cons_sublist_cons : a :: l₁ <+ a :: l₂ ↔ l₁ <+ l₂ :=
@@ -2882,7 +3031,7 @@ theorem pairwise_map {l : List α} :
     (l.map f).Pairwise R ↔ l.Pairwise fun a b => R (f a) (f b) := by
   induction l
   · simp
-  · simp only [map, pairwise_cons, forall_mem_map_iff, *]
+  · simp only [map, pairwise_cons, forall_mem_map, *]
 
 theorem pairwise_append {l₁ l₂ : List α} :
     (l₁ ++ l₂).Pairwise R ↔ l₁.Pairwise R ∧ l₂.Pairwise R ∧ ∀ a ∈ l₁, ∀ b ∈ l₂, R a b := by
